done/Iron/Language/SystemF2Effect/Step/TypeC.v
@@ -7,7 +7,7 @@ Require Export Iron.Language.SystemF2Effect.Step.TypeF.
 
 (********************************************************************)
 (* Type of an expression in a frame context. *)
-Inductive TYPEC 
+Inductive TypeC 
    :  kienv -> tyenv 
    -> stenv -> stprops 
    -> stack -> exp 
@@ -15,17 +15,17 @@ Inductive TYPEC
  | TcExp
    :  forall ke te se sp fs x1 t1 e1 t2 e2 e3
    ,  EquivT ke sp (TSum e1 e2) e3 KEffect
-   -> TYPEX  ke te se sp x1 t1 e1
-   -> TYPEF  ke te se sp fs t1 t2 e2
-   -> TYPEC  ke te se sp fs x1 t2 e3.
+   -> TypeX  ke te se sp x1 t1 e1
+   -> TypeF  ke te se sp fs t1 t2 e2
+   -> TypeC  ke te se sp fs x1 t2 e3.
 
-Hint Constructors TYPEC.
+Hint Constructors TypeC.
 
 
 Ltac inverts_typec :=
  repeat
   (try (match goal with
-        | [H: TYPEC _ _ _ _ _ _ _ _ |- _ ] => inverts H
+        | [H: TypeC _ _ _ _ _ _ _ _ |- _ ] => inverts H
         end);
    try inverts_typef).
 
@@ -33,7 +33,7 @@ Ltac inverts_typec :=
 (********************************************************************)
 Lemma typeC_kindT_effect
  :  forall ke te se sp fs x t e
- ,  TYPEC  ke te se sp fs x t e
+ ,  TypeC  ke te se sp fs x t e
  -> KindT  ke sp e KEffect.
 Proof.
  intros.
