done/Iron/Language/SystemF2Effect/Store/StoreM.v
@@ -7,19 +7,19 @@ Require Export Iron.Language.SystemF2Effect.Store.Bind.
    All types in the store typing have a corresponding binding in the store.
    We don't want entries in the store typing that don't have corresponding
    bindings in the store. *)
-Definition STOREM (se: stenv) (ss: store)
+Definition StoreM (se: stenv) (ss: store)
  := length se = length ss.
-Hint Unfold STOREM.
+Hint Unfold StoreM.
 
 
 (* Extended store environment models the extended store *)
 Lemma storeM_snoc
  :  forall se ss t stv
- ,  STOREM se ss
- -> STOREM (t <: se) (stv <: ss).
+ ,  StoreM se ss
+ -> StoreM (t <: se) (stv <: ss).
 Proof.
  intros.
- unfold STOREM.
+ unfold StoreM.
  have (length se = length ss). 
  burn.
 Qed.
