done/Iron/Language/SystemF2Effect/Store/StoreP.v
@@ -10,7 +10,7 @@ Require Export Iron.Language.SystemF2Effect.Store.Bind.
    the frame stack. This is because we need to be able to pop a Priv frame
    and still have any region handles in the expression being well typed,
    along with dangling references into that region. *)
-Definition STOREP  (sp : stprops) (fs : stack)
+Definition StoreP  (sp : stprops) (fs : stack)
  := (forall m1 p2, In (FPriv  m1       p2) fs -> In (SRegion p2) sp)
  /\ (forall p1 p2, In (FPriv (Some p1) p2) fs -> In (SRegion p1) sp).
 
@@ -18,10 +18,10 @@ Definition STOREP  (sp : stprops) (fs : stack)
 (* Weaken frame stack in store properties. *)
 Lemma storeP_snoc
  :  forall sp fs p
- ,  STOREP sp fs
- -> STOREP (SRegion p <: sp) (fs :> FPriv None p).
+ ,  StoreP sp fs
+ -> StoreP (SRegion p <: sp) (fs :> FPriv None p).
 Proof.
- unfold STOREP in *. rip.
+ unfold StoreP in *. rip.
  - inverts H0. inverts H.
    + eauto.
    + have HN: (p = p2 \/ ~(p = p2)).
@@ -33,21 +33,21 @@ Hint Resolve storeP_snoc.
 
 Lemma storeP_stprops_snoc
  :  forall sp fs p
- ,  STOREP sp fs
- -> STOREP (p <: sp) fs.
+ ,  StoreP sp fs
+ -> StoreP (p <: sp) fs.
 Proof.
- unfold STOREP in *. rip; eauto.
+ unfold StoreP in *. rip; eauto.
 Qed.
 Hint Resolve storeP_stprops_snoc.
 
 
 Lemma storeP_pop
  :  forall sp fs f
- ,  STOREP sp (fs :> f)
- -> STOREP sp fs.
+ ,  StoreP sp (fs :> f)
+ -> StoreP sp fs.
 Proof.
  intros.
- unfold STOREP in *.
+ unfold StoreP in *.
  firstorder.
 Qed.
 Hint Resolve storeP_pop.
