done/Iron/Language/SystemF2Effect/Store/TypeB.v
@@ -4,15 +4,15 @@ Require Export Iron.Language.SystemF2Effect.Store.Bind.
 
 (******************************************************************************)
 (* Types of store bindings. *)
-Inductive TYPEB : kienv -> tyenv -> stenv -> stprops -> stbind -> ty -> Prop := 
+Inductive TypeB : kienv -> tyenv -> stenv -> stprops -> stbind -> ty -> Prop := 
  (* A store binding that contains a live value.
     Requiring that the region handle is well kinded ensures that it's 
     mentioned in the store properties. *)
  | TbValue
    :  forall ke te se sp n v t
    ,  KindT  ke sp (TRgn n) KRegion
-   -> TYPEV  ke te se sp v t
-   -> TYPEB  ke te se sp (StValue n v) (TRef (TRgn n) t)
+   -> TypeV  ke te se sp v t
+   -> TypeB  ke te se sp (StValue n v) (TRef (TRgn n) t)
 
  (* After a store binding has been dealloated,
     we can treat the location has having any type we want.
@@ -21,18 +21,18 @@ Inductive TYPEB : kienv -> tyenv -> stenv -> stprops -> stbind -> ty -> Prop :=
  | TbDead 
    :  forall ke te se sp n t
    ,  KindT  ke sp (TRgn n) KRegion
-   -> TYPEB  ke te se sp (StDead n)    (TRef (TRgn n) t).
+   -> TypeB  ke te se sp (StDead n)    (TRef (TRgn n) t).
 
-Hint Constructors TYPEB.
+Hint Constructors TypeB.
 
 
 (******************************************************************************)
 (* Weakening store environment in type of store binding *)
 Lemma typeB_stenv_snoc 
  :  forall ke te se sp v t1 t2 
- ,  TYPEB  ke te se sp v t1
+ ,  TypeB  ke te se sp v t1
  -> ClosedT t2
- -> TYPEB  ke te (t2 <: se) sp v t1.
+ -> TypeB  ke te (t2 <: se) sp v t1.
 Proof.
  intros. 
  inverts H; eauto.
@@ -43,8 +43,8 @@ Hint Resolve typeB_stenv_snoc.
 (* Weakening store properties  in type of store binding *)
 Lemma typeB_stprops_snoc
  :  forall ke te se sp v t p
- ,  TYPEB  ke te se sp v t
- -> TYPEB  ke te se (p <: sp) v t.
+ ,  TypeB  ke te se sp v t
+ -> TypeB  ke te se (p <: sp) v t.
 Proof. 
  intros. 
  inverts H; eauto using kind_stprops_snoc.
@@ -54,8 +54,8 @@ Hint Resolve typeB_stprops_snoc.
 
 Lemma typeB_stprops_cons
  :  forall ke te se sp v t p
- ,  TYPEB  ke te se sp v t
- -> TYPEB  ke te se (sp :> p) v t.
+ ,  TypeB  ke te se sp v t
+ -> TypeB  ke te se (sp :> p) v t.
 Proof. 
  intros.
  inverts H; eauto using kind_stprops_cons.
@@ -66,8 +66,8 @@ Hint Resolve typeB_stprops_snoc.
 Lemma typeB_mergeT
  :  forall ke te se sp b t p1 p2
  ,  In (SRegion p1) sp
- -> TYPEB  ke te se sp b t
- -> TYPEB  ke (mergeTE p1 p2 te) (mergeTE p1 p2 se) sp 
+ -> TypeB  ke te se sp b t
+ -> TypeB  ke (mergeTE p1 p2 te) (mergeTE p1 p2 se) sp 
               (mergeB p1 p2 b) (mergeT p1 p2 t).
 Proof.
  intros.
