done/Iron/Language/SystemF2Effect/Store.v
@@ -11,13 +11,13 @@ Require Export Iron.Language.SystemF2Effect.Store.LiveS.
    the store environment *)
 Lemma storet_get_typev
  :  forall se sp ss ix r v t
- ,  STORET se sp ss
+ ,  StoreT se sp ss
  -> get ix se = Some (TRef (TRgn r) t)
  -> get ix ss = Some (StValue r v)
- -> TYPEV nil nil se sp v t.
+ -> TypeV nil nil se sp v t.
 Proof.
  intros.
- unfold STORET in *.
+ unfold StoreT in *.
  lets D: (@Forall2_get_get_same stbind ty) H1 H0. eauto.
  inverts D. auto.
 Qed.
