done/Iron/Language/SystemF2Effect/Store/Wf.v
@@ -13,8 +13,8 @@ Inductive WfS   : stenv -> stprops -> store -> Prop :=
  | WfS_
    :  forall se sp ss
    ,  Forall ClosedT se
-   -> STOREM se    ss
-   -> STORET se sp ss
+   -> StoreM se    ss
+   -> StoreT se sp ss
    -> WfS se sp ss.
 Hint Constructors WfS.
 
@@ -24,9 +24,9 @@ Inductive WfFS : stenv -> stprops -> store -> stack -> Prop :=
  | WfFS_
    :  forall se sp ss fs
    ,  Forall ClosedT se
-   -> STOREM se ss
-   -> STORET se sp ss
-   -> STOREP sp fs
+   -> StoreM se ss
+   -> StoreT se sp ss
+   -> StoreP sp fs
    -> WfFS se sp ss fs.
 Hint Constructors WfFS.
 
@@ -54,7 +54,7 @@ Lemma wfFS_typeb
  :  forall se sp ss fs b
  ,  WfFS se sp ss fs
  -> In b ss
- -> (exists t, TYPEB nil nil se sp b t).
+ -> (exists t, TypeB nil nil se sp b t).
 Proof. 
  intros.
  inverts H. 
@@ -106,7 +106,7 @@ Lemma wfFS_push_priv_ext
 Proof.
  intros.
  inverts H1. eapply WfFS_; rip.
- unfold STOREP in *. rip.
+ unfold StoreP in *. rip.
  - inverts H1; eauto. 
    inverts H5. eauto.
  - inverts H1; eauto.
@@ -118,8 +118,8 @@ Hint Resolve wfFS_push_priv_ext.
 (* Deallocating a region preserves well-formedness of the store. *)
 Lemma typeB_deallocate
  :  forall ke te se sp p b t
- ,  TYPEB  ke te se sp b t
- -> TYPEB  ke te se sp (deallocRegion p b) t.
+ ,  TypeB  ke te se sp b t
+ -> TypeB  ke te se sp (deallocRegion p b) t.
 Proof.
  intros.
  destruct b.
@@ -132,11 +132,11 @@ Qed.
 (* Deallocating bindings preserves the well typedness of the store. *)
 Lemma storeT_deallocate
  :  forall se sp ss p
- ,  STORET se sp ss
- -> STORET se sp (map (deallocRegion p) ss).
+ ,  StoreT se sp ss
+ -> StoreT se sp (map (deallocRegion p) ss).
 Proof.
  intros.
- unfold STORET in *.
+ unfold StoreT in *.
  eapply Forall2_map_left.
  eapply Forall2_impl.
  - intros.
@@ -154,10 +154,10 @@ Lemma wfFS_region_deallocate
 Proof.
  intros.
  inverts H. eapply WfFS_; rip.
- - unfold STOREM in *.
+ - unfold StoreM in *.
    rewrite map_length; auto.
  - eapply storeT_deallocate; auto.
- - unfold STOREP in *; snorm; eauto.
+ - unfold StoreP in *; snorm; eauto.
 Qed.
 
 
@@ -174,12 +174,12 @@ Proof.
    + intros. eapply mergeT_wfT; eauto.
    + auto.
 
- - unfold STOREM in *.
+ - unfold StoreM in *.
    unfold mergeTE. 
    unfold mergeBs.
    repeat (rewrite map_length). auto.
 
- - unfold STORET.
+ - unfold StoreT.
    eapply storeT_mergeB; auto.
    
  - eapply storeP_pop; eauto.
@@ -191,7 +191,7 @@ Qed.
 Lemma wfFS_stbind_snoc
  :  forall se sp ss fs p v t
  ,  KindT  nil sp (TRgn p) KRegion
- -> TYPEV  nil nil se sp v t
+ -> TypeV  nil nil se sp v t
  -> WfFS           se sp ss fs
  -> WfFS   (TRef (TRgn p) t <: se) sp 
            (StValue p v <: ss) fs.
@@ -219,17 +219,17 @@ Lemma wfFS_stbind_update
  :  forall se sp ss fs l p v t
  ,  get l se = Some (TRef (TRgn p) t)
  -> KindT nil sp (TRgn p) KRegion
- -> TYPEV nil nil se sp v t
+ -> TypeV nil nil se sp v t
  -> WfFS se sp ss fs
  -> WfFS se sp (update l (StValue p v) ss) fs.
 Proof.
  intros se sp ss fs l p v t HG HK HV HWF1.
  inverts HWF1. eapply WfFS_; rip.
  - have (length se = length ss).
-   unfold STOREM.
+   unfold StoreM.
    rewritess.
    rewrite update_length. auto.
- - unfold STORET.
+ - unfold StoreT.
    eapply Forall2_update_right; eauto.
 Qed.
 
