done/Iron/Language/SystemF2Effect/Value/Relation/TyJudge.v
@@ -23,7 +23,7 @@ Fixpoint typeOfOp1 (op : op1) : ty
 
 (* Types of Value expressions *)
 Inductive 
-  TYPEV : kienv -> tyenv -> stenv -> stprops 
+  TypeV : kienv -> tyenv -> stenv -> stprops 
         -> val  -> ty 
         -> Prop := 
 
@@ -33,7 +33,7 @@ Inductive
     :  forall ke te se sp i t
     ,  get i te = Some t
     -> KindT  ke sp t KData
-    -> TYPEV  ke te se sp (VVar i) t 
+    -> TypeV  ke te se sp (VVar i) t 
 
   (* Store locations.
      We get the type of a location from the store typing.
@@ -44,7 +44,7 @@ Inductive
     :  forall ke te se sp l r t
     ,  get l se = Some (TRef r t)
     -> KindT  ke sp       (TRef r t) KData       
-    -> TYPEV  ke te se sp (VLoc l)   (TRef r t)
+    -> TypeV  ke te se sp (VLoc l)   (TRef r t)
 
   (* Value abstraction.
      The body is checked in an environment extended with the type of
@@ -52,8 +52,8 @@ Inductive
   | TvLam
     :  forall ke te se sp t1 t2 x2 e2
     ,  KindT  ke sp t1 KData
-    -> TYPEX  ke (te :> t1) se sp x2 t2 e2
-    -> TYPEV  ke te         se sp (VLam t1 x2) (TFun t1 e2 t2)
+    -> TypeX  ke (te :> t1) se sp x2 t2 e2
+    -> TypeV  ke te         se sp (VLam t1 x2) (TFun t1 e2 t2)
 
   (* Type abstraction.
      The body is checked in an environemnt extended with the kind of
@@ -66,8 +66,8 @@ Inductive
      annotation. *) 
   | TvLAM
     :  forall ke te se sp k1 t2 x2
-    ,  TYPEX (ke :> k1) (liftTE 0 te) (liftTE 0 se) sp x2 t2 (TBot KEffect)
-    -> TYPEV ke          te            se   sp (VLAM k1 x2) (TForall k1 t2)
+    ,  TypeX (ke :> k1) (liftTE 0 te) (liftTE 0 se) sp x2 t2 (TBot KEffect)
+    -> TypeV ke          te            se   sp (VLAM k1 x2) (TForall k1 t2)
 
   (* Primitive constants. 
      We get the types of these from the 'typeOfConst' function so we can
@@ -75,10 +75,10 @@ Inductive
   | TvConst
     :  forall ke te se sp c t
     ,  t = typeOfConst c
-    -> TYPEV  ke te se sp (VConst c) t
+    -> TypeV  ke te se sp (VConst c) t
 
 
-  with TYPEX :  kienv -> tyenv -> stenv -> stprops 
+  with TypeX :  kienv -> tyenv -> stenv -> stprops 
              -> exp   -> ty -> ty 
              -> Prop :=
 
@@ -87,30 +87,30 @@ Inductive
      in turn means they can't perform any more effectful actions. *)
   | TxVal
     :  forall ke te se sp v1 t1
-    ,  TYPEV  ke te se sp v1 t1
-    -> TYPEX  ke te se sp (XVal v1) t1 (TBot KEffect)
+    ,  TypeV  ke te se sp v1 t1
+    -> TypeX  ke te se sp (XVal v1) t1 (TBot KEffect)
 
   (* Let-bindings. *)
   | TxLet
     :  forall ke te se sp t1 x1 t2 x2 e1 e2
     ,  KindT  ke sp t1 KData
-    -> TYPEX  ke te         se sp x1 t1 e1
-    -> TYPEX  ke (te :> t1) se sp x2 t2 e2
-    -> TYPEX  ke te         se sp (XLet t1 x1 x2) t2 (TSum e1 e2)
+    -> TypeX  ke te         se sp x1 t1 e1
+    -> TypeX  ke (te :> t1) se sp x2 t2 e2
+    -> TypeX  ke te         se sp (XLet t1 x1 x2) t2 (TSum e1 e2)
 
   (* Value application. *)
   | TxApp
     :  forall ke te se sp t11 t12 v1 v2 e1
-    ,  TYPEV  ke te se sp v1 (TFun t11 e1 t12) 
-    -> TYPEV  ke te se sp v2 t11
-    -> TYPEX  ke te se sp (XApp v1 v2) t12 e1
+    ,  TypeV  ke te se sp v1 (TFun t11 e1 t12) 
+    -> TypeV  ke te se sp v2 t11
+    -> TypeX  ke te se sp (XApp v1 v2) t12 e1
 
   (* Type application. *)
   | TvAPP
     :  forall ke te se sp v1 k11 t12 t2
-    ,  TYPEV  ke te se sp v1 (TForall k11 t12)
+    ,  TypeV  ke te se sp v1 (TForall k11 t12)
     -> KindT  ke sp t2 k11
-    -> TYPEX  ke te se sp (XAPP v1 t2) (substTT 0 t2 t12) (TBot KEffect)
+    -> TypeX  ke te se sp (XAPP v1 t2) (substTT 0 t2 t12) (TBot KEffect)
 
   (* Store Operators ******************)
   (* Create a private region. *)
@@ -118,48 +118,48 @@ Inductive
     :  forall ke te se sp x t tL e eL
     ,  lowerTT 0 t                = Some tL
     -> lowerTT 0 (maskOnVarT 0 e) = Some eL
-    -> TYPEX (ke :> KRegion) (liftTE 0 te) (liftTE 0 se) sp x            t  e
-    -> TYPEX ke              te            se            sp (XPrivate x) tL eL
+    -> TypeX (ke :> KRegion) (liftTE 0 te) (liftTE 0 se) sp x            t  e
+    -> TypeX ke              te            se            sp (XPrivate x) tL eL
 
   (* Extend an existing region. *)
   | TxExtend
     :  forall ke te se sp r1 x2 t e eL
     ,  lowerTT 0 (maskOnVarT 0 e) = Some eL
     -> KindT ke sp r1 KRegion
-    -> TYPEX (ke :> KRegion) (liftTE 0 te) (liftTE 0 se) sp x2 t e
-    -> TYPEX ke te se  sp (XExtend r1 x2) (substTT 0 r1 t) (TSum eL (TAlloc r1))
+    -> TypeX (ke :> KRegion) (liftTE 0 te) (liftTE 0 se) sp x2 t e
+    -> TypeX ke te se  sp (XExtend r1 x2) (substTT 0 r1 t) (TSum eL (TAlloc r1))
 
   (* Allocate a new heap binding. *)
   | TxOpAlloc 
     :  forall ke te se sp r1 v2 t2
     ,  KindT  ke sp r1 KRegion
-    -> TYPEV  ke te se sp v2 t2
-    -> TYPEX  ke te se sp (XAlloc r1 v2) (TRef r1 t2) (TAlloc r1)
+    -> TypeV  ke te se sp v2 t2
+    -> TypeX  ke te se sp (XAlloc r1 v2) (TRef r1 t2) (TAlloc r1)
 
   (* Read a value from a heap binding. *)
   | TxOpRead
     :  forall ke te se sp v1 r1 t2
     ,  KindT  ke sp r1 KRegion
-    -> TYPEV  ke te se sp v1 (TRef r1 t2)
-    -> TYPEX  ke te se sp (XRead r1 v1)     t2    (TRead r1)
+    -> TypeV  ke te se sp v1 (TRef r1 t2)
+    -> TypeX  ke te se sp (XRead r1 v1)     t2    (TRead r1)
 
   (* Write a value to a heap binding. *)
   | TxOpWrite
     :  forall ke te se sp v1 v2 r1 t2
     ,  KindT  ke sp r1 KRegion
-    -> TYPEV  ke te se sp v1 (TRef r1 t2)
-    -> TYPEV  ke te se sp v2 t2
-    -> TYPEX  ke te se sp (XWrite r1 v1 v2) TUnit (TWrite r1)
+    -> TypeV  ke te se sp v1 (TRef r1 t2)
+    -> TypeV  ke te se sp v2 t2
+    -> TypeX  ke te se sp (XWrite r1 v1 v2) TUnit (TWrite r1)
 
   (* Primtive Operators ***************)
   | TxOpPrim
     :  forall ke te se sp op v1 t11 t12 e
     ,  typeOfOp1 op = TFun t11 t12 e
-    -> TYPEV  ke te se sp v1 t11
-    -> TYPEX  ke te se sp (XOp1 op v1) t12 e.
+    -> TypeV  ke te se sp v1 t11
+    -> TypeX  ke te se sp (XOp1 op v1) t12 e.
 
-Hint Constructors TYPEV.
-Hint Constructors TYPEX.
+Hint Constructors TypeV.
+Hint Constructors TypeX.
 
 
 (********************************************************************)
@@ -167,21 +167,21 @@ Hint Constructors TYPEX.
 Ltac inverts_type :=
  repeat 
   (match goal with 
-   | [ H: TYPEV _ _ _ _ (VVar   _)     _    |- _ ] => inverts H
-   | [ H: TYPEV _ _ _ _ (VLoc   _)     _    |- _ ] => inverts H
-   | [ H: TYPEV _ _ _ _ (VLam   _ _)   _    |- _ ] => inverts H
-   | [ H: TYPEV _ _ _ _ (VLAM   _ _)   _    |- _ ] => inverts H
-   | [ H: TYPEV _ _ _ _ (VConst _)     _    |- _ ] => inverts H
-   | [ H: TYPEX _ _ _ _ (XVal   _)     _ _  |- _ ] => inverts H
-   | [ H: TYPEX _ _ _ _ (XLet   _ _ _) _ _  |- _ ] => inverts H 
-   | [ H: TYPEX _ _ _ _ (XApp   _ _)   _ _  |- _ ] => inverts H 
-   | [ H: TYPEX _ _ _ _ (XAPP   _ _)   _ _  |- _ ] => inverts H 
-   | [ H: TYPEX _ _ _ _ (XPrivate _)   _ _  |- _ ] => inverts H
-   | [ H: TYPEX _ _ _ _ (XExtend  _ _) _ _  |- _ ] => inverts H
-   | [ H: TYPEX _ _ _ _ (XAlloc _ _)   _ _  |- _ ] => inverts H
-   | [ H: TYPEX _ _ _ _ (XRead  _ _)   _ _  |- _ ] => inverts H
-   | [ H: TYPEX _ _ _ _ (XWrite _ _ _) _ _  |- _ ] => inverts H
-   | [ H: TYPEX _ _ _ _ (XOp1   _ _)   _ _  |- _ ] => inverts H 
+   | [ H: TypeV _ _ _ _ (VVar   _)     _    |- _ ] => inverts H
+   | [ H: TypeV _ _ _ _ (VLoc   _)     _    |- _ ] => inverts H
+   | [ H: TypeV _ _ _ _ (VLam   _ _)   _    |- _ ] => inverts H
+   | [ H: TypeV _ _ _ _ (VLAM   _ _)   _    |- _ ] => inverts H
+   | [ H: TypeV _ _ _ _ (VConst _)     _    |- _ ] => inverts H
+   | [ H: TypeX _ _ _ _ (XVal   _)     _ _  |- _ ] => inverts H
+   | [ H: TypeX _ _ _ _ (XLet   _ _ _) _ _  |- _ ] => inverts H 
+   | [ H: TypeX _ _ _ _ (XApp   _ _)   _ _  |- _ ] => inverts H 
+   | [ H: TypeX _ _ _ _ (XAPP   _ _)   _ _  |- _ ] => inverts H 
+   | [ H: TypeX _ _ _ _ (XPrivate _)   _ _  |- _ ] => inverts H
+   | [ H: TypeX _ _ _ _ (XExtend  _ _) _ _  |- _ ] => inverts H
+   | [ H: TypeX _ _ _ _ (XAlloc _ _)   _ _  |- _ ] => inverts H
+   | [ H: TypeX _ _ _ _ (XRead  _ _)   _ _  |- _ ] => inverts H
+   | [ H: TypeX _ _ _ _ (XWrite _ _ _) _ _  |- _ ] => inverts H
+   | [ H: TypeX _ _ _ _ (XOp1   _ _)   _ _  |- _ ] => inverts H 
    end).
 
 
