done/Iron/Language/SystemF2Effect/Value/Relation/TyJudge/TypeKind.v
@@ -4,13 +4,13 @@ Require Import Iron.Language.SystemF2Effect.Value.Relation.TyJudge.
 
 Lemma typex_kind_type_effect
  :  forall ke te se sp v t e
- ,  TYPEX  ke te se sp v t e
+ ,  TypeX  ke te se sp v t e
  -> (KindT ke sp t KData /\ KindT ke sp e KEffect).
 Proof.
  intros. gen ke te se sp t e. 
  induction v using exp_mutind with
   (PV := fun v => forall ke te se sp t
-      ,  TYPEV  ke te se sp v t
+      ,  TypeV  ke te se sp v t
       -> KindT  ke sp t KData);
    intros; inverts_type; eauto 1.
 
@@ -91,7 +91,7 @@ Hint Resolve typex_kind_type_effect.
 
 Lemma typev_kind_type
  :  forall ke te se sp v t
- ,  TYPEV  ke te se sp v t
+ ,  TypeV  ke te se sp v t
  -> KindT  ke sp t KData.
 Proof.
  intros.
@@ -103,7 +103,7 @@ Hint Resolve typev_kind_type.
 
 Lemma typex_kind_type
  :  forall ke te se sp x t e
- ,  TYPEX  ke te se sp x t e
+ ,  TypeX  ke te se sp x t e
  -> KindT  ke sp t KData.
 Proof. 
  intros. 
@@ -114,7 +114,7 @@ Hint Resolve typex_kind_type.
 
 Lemma typex_kind_effect
  :  forall ke te se sp x t e
- ,  TYPEX  ke te se sp x t e
+ ,  TypeX  ke te se sp x t e
  -> KindT  ke sp e KEffect.
 Proof. 
  intros. 
