done/Iron/Language/SystemF2Effect/Value/Relation/TyJudge/WeakStEnv.v
@@ -6,15 +6,15 @@ Require Import Iron.Language.SystemF2Effect.Value.Relation.TyJudge.
 Lemma typex_stenv_snoc 
  :  forall ke te se sp t2 x t1 e1
  ,  ClosedT t2
- -> TYPEX  ke te se         sp x t1 e1
- -> TYPEX  ke te (t2 <: se) sp x t1 e1.
+ -> TypeX  ke te se         sp x t1 e1
+ -> TypeX  ke te (t2 <: se) sp x t1 e1.
 Proof.
  intros. gen ke te se sp t1 e1 t2.
  induction x using exp_mutind with 
   (PV := fun v => forall ke te se sp t1 t2
       ,  ClosedT t2
-      -> TYPEV ke te se         sp v t1
-      -> TYPEV ke te (t2 <: se) sp v t1)
+      -> TypeV ke te se         sp v t1
+      -> TypeV ke te (t2 <: se) sp v t1)
   ; intros; inverts_type; eauto.
 
  - Case "VLAM".
@@ -47,11 +47,11 @@ Hint Resolve typex_stenv_snoc.
 Lemma typev_stenv_snoc
  :  forall ke te se sp t2 v t1
  ,  ClosedT t2
- -> TYPEV ke te se         sp v t1
- -> TYPEV ke te (t2 <: se) sp v t1.
+ -> TypeV ke te se         sp v t1
+ -> TypeV ke te (t2 <: se) sp v t1.
 Proof.
  intros.
- have HX: (TYPEX ke te se sp (XVal v) t1 (TBot KEffect)).
+ have HX: (TypeX ke te se sp (XVal v) t1 (TBot KEffect)).
  eapply typex_stenv_snoc in HX.
  inverts HX; eauto.
  eauto.
@@ -62,8 +62,8 @@ Hint Resolve typev_stenv_snoc.
 Lemma typex_stenv_weaken
  :  forall ke te se1 se2 sp x t1 e1
  ,  Forall ClosedT se2
- -> TYPEX  ke te  se1         sp x t1 e1
- -> TYPEX  ke te (se2 >< se1) sp x t1 e1.
+ -> TypeX  ke te  se1         sp x t1 e1
+ -> TypeX  ke te (se2 >< se1) sp x t1 e1.
 Proof.
  intros. gen ke te se1 sp.
  induction se2; intros.
@@ -78,8 +78,8 @@ Lemma typex_stenv_extends
  :  forall ke te se1 se2 sp x t1 e1
  ,  Forall ClosedT se2
  -> extends se2 se1
- -> TYPEX ke te se1 sp x t1 e1
- -> TYPEX ke te se2 sp x t1 e1.
+ -> TypeX ke te se1 sp x t1 e1
+ -> TypeX ke te se2 sp x t1 e1.
 Proof.
  intros.
  unfold extends in *.
@@ -94,13 +94,13 @@ Lemma typev_stenv_extends
  :  forall ke te sp se1 se2 v t1
  ,  Forall ClosedT se2
  -> extends se2 se1
- -> TYPEV ke te se1 sp v t1
- -> TYPEV ke te se2 sp v t1.
+ -> TypeV ke te se1 sp v t1
+ -> TypeV ke te se2 sp v t1.
 Proof.
  intros.
  unfold extends in *.
  destruct H0 as [se3]. subst.
- assert (TYPEX ke te (se3 >< se1) sp (XVal v) t1 (TBot KEffect)) as HX.
+ assert (TypeX ke te (se3 >< se1) sp (XVal v) t1 (TBot KEffect)) as HX.
   eauto.
  inverts HX. auto.
 Qed.
