done/Iron/Language/SystemF2Effect/Value/Relation/TyJudge/WeakStProps.v
@@ -5,14 +5,14 @@ Require Import Iron.Language.SystemF2Effect.Value.Relation.TyJudge.
 (* Weakening Store Properties in Type Judgement *)
 Lemma typex_stprops_snoc
  :  forall ke te se sp x t e p
- ,  TYPEX  ke te se sp        x t e
- -> TYPEX  ke te se (p <: sp) x t e.
+ ,  TypeX  ke te se sp        x t e
+ -> TypeX  ke te se (p <: sp) x t e.
 Proof.
  intros. gen ke te se sp t e p.
  induction x using exp_mutind with 
   (PV := fun v => forall ke te se sp t p
-      ,  TYPEV ke te se sp v t
-      -> TYPEV ke te se (p <: sp) v t);
+      ,  TypeV ke te se sp v t
+      -> TypeV ke te se (p <: sp) v t);
   intros; inverts_type; 
   eauto using kind_stprops_snoc.
 Qed.
@@ -21,11 +21,11 @@ Hint Resolve typex_stprops_snoc.
 
 Lemma typev_stprops_snoc
  :  forall ke te se sp        v t p
- ,  TYPEV  ke te se sp        v t
- -> TYPEV  ke te se (p <: sp) v t. 
+ ,  TypeV  ke te se sp        v t
+ -> TypeV  ke te se (p <: sp) v t. 
 Proof.
  intros.
- have HX: (TYPEX ke te se (p <: sp) (XVal v) t (TBot KEffect)).
+ have HX: (TypeX ke te se (p <: sp) (XVal v) t (TBot KEffect)).
  inverts HX.
  trivial.
 Qed.
@@ -34,14 +34,14 @@ Hint Resolve typev_stprops_snoc.
 
 Lemma typex_stprops_cons
  :  forall ke te se sp x t e p
- ,  TYPEX  ke te se sp        x t e
- -> TYPEX  ke te se (sp :> p) x t e.
+ ,  TypeX  ke te se sp        x t e
+ -> TypeX  ke te se (sp :> p) x t e.
 Proof.
  intros. gen ke te se sp t e p.
  induction x using exp_mutind with 
   (PV := fun v => forall ke te se sp t p
-      ,  TYPEV ke te se sp v t
-      -> TYPEV ke te se (sp :> p) v t);
+      ,  TypeV ke te se sp v t
+      -> TypeV ke te se (sp :> p) v t);
   intros; inverts_type; 
   eauto using kind_stprops_cons.
 Qed.
@@ -50,11 +50,11 @@ Hint Resolve typex_stprops_cons.
 
 Lemma typev_stprops_cons
  :  forall ke te se sp v t p
- ,  TYPEV  ke te se sp v t
- -> TYPEV  ke te se (sp :> p) v t.
+ ,  TypeV  ke te se sp v t
+ -> TypeV  ke te se (sp :> p) v t.
 Proof.
  intros.
- have HX: (TYPEX ke te se (sp :> p) (XVal v) t (TBot KEffect)).
+ have HX: (TypeX ke te se (sp :> p) (XVal v) t (TBot KEffect)).
  inverts HX.
  trivial.
 Qed.
@@ -63,8 +63,8 @@ Hint Resolve typev_stprops_cons.
 
 Lemma typex_stprops_weaken
  :  forall ke te se sp1 sp2 x t e
- ,  TYPEX  ke te se sp1          x t e
- -> TYPEX  ke te se (sp2 >< sp1) x t e.
+ ,  TypeX  ke te se sp1          x t e
+ -> TypeX  ke te se (sp2 >< sp1) x t e.
 Proof.
  intros. gen ke te se sp1 t e.
  induction sp2; intros; burn.
@@ -77,8 +77,8 @@ Hint Resolve typex_stprops_weaken.
 Lemma typex_stprops_extends
  :  forall ke te se sp1 sp2 x t e
  ,  extends sp2 sp1
- -> TYPEX  ke te se sp1 x t e
- -> TYPEX  ke te se sp2 x t e.
+ -> TypeX  ke te se sp1 x t e
+ -> TypeX  ke te se sp2 x t e.
 Proof.
  intros.
  unfold extends in *.
@@ -91,13 +91,13 @@ Hint Resolve typex_stprops_extends.
 Lemma typev_stprops_extends
  :  forall ke te se sp1 sp2 v t
  ,  extends sp2 sp1 
- -> TYPEV ke te se sp1 v t
- -> TYPEV ke te se sp2 v t.
+ -> TypeV ke te se sp1 v t
+ -> TypeV ke te se sp2 v t.
 Proof.
  intros.
  unfold extends in *.
  destruct H as [sp3]. subst.
- have HX: (TYPEX ke te se (sp3 >< sp1) (XVal v) t (TBot KEffect)).
+ have HX: (TypeX ke te se (sp3 >< sp1) (XVal v) t (TBot KEffect)).
  inverts HX.
  eauto.
 Qed.
