done/Iron/Language/SystemF2Effect/Value/Relation/TyJudge/Wf.v
@@ -5,13 +5,13 @@ Require Export Iron.Language.SystemF2Effect.Value.Relation.TyJudge.
 (* A well typed expression is well formed *)
 Lemma typex_wfX
  :  forall ke te se sp x t e
- ,  TYPEX  ke te se sp x t e
+ ,  TypeX  ke te se sp x t e
  -> wfX (length ke) (length te) (length se) x.
 Proof.
  intros. gen ke te se sp t e.
  induction x using exp_mutind with 
   (PV := fun v => forall ke te se sp t1
-      ,  TYPEV ke te se sp v t1
+      ,  TypeV ke te se sp v t1
       -> wfV (length ke) (length te) (length se) v);
    rip; inverts_type; try burn.
 
